swap uses bspec contract without high-level step

examples/riscv/swap/swap_specScript.sml
@@ -8,7 +8,6 @@ open bir_programSyntax bir_program_labelsTheory;
 open bir_immTheory bir_valuesTheory bir_expTheory bir_exp_immTheory;
 open bir_tsTheory bir_bool_expTheory bir_programTheory;
 
-
 open bir_riscv_backlifterTheory;
 open bir_backlifterLib;
 open bir_riscv_extrasTheory;
@@ -50,23 +49,6 @@ open swapTheory;
 
 val _ = new_theory "swap_spec";
 
-Definition swap_mem_spec_def:
- swap_mem_spec ms =
- let ms'_mem8 = (riscv_mem_store_dword (ms.c_gpr ms.procID 0w)
-   (riscv_mem_load_dword ms.MEM8 (ms.c_gpr ms.procID 1w)) ms.MEM8)
- in
-   (riscv_mem_store_dword (ms.c_gpr ms.procID 1w)
-    (riscv_mem_load_dword ms.MEM8 (ms.c_gpr ms.procID 0w)) ms'_mem8)
-End
-
-Definition swap_spec_output_def:
- swap_spec_output ms : riscv_state = ms with MEM8 := swap_mem_spec ms
-End
-
-Definition swap_spec_def:
- swap_spec ms ms' : bool = (ms'.MEM8 = swap_mem_spec ms)
-End
-
 (* --------------- *)
 (* RISC-V contract *)
 (* --------------- *)
@@ -87,7 +69,11 @@ Definition riscv_swap_post_def:
    riscv_mem_load_dword m.MEM8 y = xv)
 End
 
-val bir_swap_pre_tm = bslSyntax.bandl [
+(* -------------- *)
+(* BSPEC contract *)
+(* -------------- *)
+
+val bspec_swap_pre_tm = bslSyntax.bandl [
  mem_addrs_aligned_prog_disj_tm "x10",
  mem_addrs_aligned_prog_disj_tm "x11",
  ``BExp_BinPred
@@ -114,135 +100,102 @@ val bir_swap_pre_tm = bslSyntax.bandl [
      (BExp_Const (Imm64 yv))`` 
 ];
 
-Definition bir_swap_pre_def:
-  bir_swap_pre x y xv yv : bir_exp_t =
-   ^bir_swap_pre_tm
+Definition bspec_swap_pre_def:
+  bspec_swap_pre x y xv yv : bir_exp_t =
+   ^bspec_swap_pre_tm
 End
 
-Definition bir_swap_post_def:
- bir_swap_post x y xv yv : bir_exp_t = 
-  BExp_BinExp BIExp_And
-   (BExp_BinPred
+val bspec_swap_post_tm = bslSyntax.bandl [
+ ``BExp_BinPred
     BIExp_Equal
     (BExp_Load
      (BExp_Den (BVar "MEM8" (BType_Mem Bit64 Bit8)))
      (BExp_Const (Imm64 x))
      BEnd_LittleEndian Bit64)
-    (BExp_Const (Imm64 yv)))
-   (BExp_BinPred
+    (BExp_Const (Imm64 yv))``,
+ ``BExp_BinPred
     BIExp_Equal
     (BExp_Load
      (BExp_Den (BVar "MEM8" (BType_Mem Bit64 Bit8)))
      (BExp_Const (Imm64 y))
      BEnd_LittleEndian Bit64)
-    (BExp_Const (Imm64 xv)))
+    (BExp_Const (Imm64 xv))``
+];
+
+Definition bspec_swap_post_def:
+ bspec_swap_post x y xv yv : bir_exp_t = 
+  ^bspec_swap_post_tm
 End
 
-(* ----------------------------------- *)
-(* Connecting RISC-V and BIR contracts *)
-(* ----------------------------------- *)
+(* ------------------------------------- *)
+(* Connecting RISC-V and BSPEC contracts *)
+(* ------------------------------------- *)
 
-Theorem swap_riscv_pre_imp_bir_pre_thm:
+Theorem swap_riscv_pre_imp_bspec_pre_thm:
  bir_pre_riscv_to_bir
   (riscv_swap_pre pre_x10 pre_x11 pre_x10_mem_deref pre_x11_mem_deref)
-  (bir_swap_pre pre_x10 pre_x11 pre_x10_mem_deref pre_x11_mem_deref)
+  (bspec_swap_pre pre_x10 pre_x11 pre_x10_mem_deref pre_x11_mem_deref)
 Proof
-  rw [bir_pre_riscv_to_bir_def] >- (
-        rw [bir_swap_pre_def] >>
-        FULL_SIMP_TAC (std_ss++HolBASimps.bir_is_bool_ss) [bir_extra_expsTheory.BExp_Aligned_def] >>
-        FULL_SIMP_TAC (std_ss++HolBASimps.bir_is_bool_ss) [bir_immTheory.n2bs_def]
-  ) >>
-    (* ++HolBACoreSimps.holBACore_ss *)
-  FULL_SIMP_TAC (std_ss) [riscv_swap_pre_def, bir_swap_pre_def, riscv_mem_load_dword_def] >>
+  rw [bir_pre_riscv_to_bir_def] >-
+   (rw [bspec_swap_pre_def] >>
+    FULL_SIMP_TAC (std_ss++HolBASimps.bir_is_bool_ss) [bir_extra_expsTheory.BExp_Aligned_def] >>
+    FULL_SIMP_TAC (std_ss++HolBASimps.bir_is_bool_ss) [bir_immTheory.n2bs_def]) >>
+  FULL_SIMP_TAC (std_ss) [riscv_swap_pre_def, bspec_swap_pre_def, riscv_mem_load_dword_def] >>
   FULL_SIMP_TAC (std_ss++pred_setSimps.PRED_SET_ss) [bir_vars_of_exp_def, bir_extra_expsTheory.BExp_Aligned_def, pred_setTheory.INSERT_UNION_EQ] >>
-
   FULL_SIMP_TAC (std_ss) [bir_env_oldTheory.bir_env_vars_are_initialised_INSERT, bir_env_oldTheory.bir_env_vars_are_initialised_EMPTY] >>
-
   FULL_SIMP_TAC (std_ss++holBACore_ss) [] >>
   PAT_X_ASSUM ``bmr_rel riscv_bmr A B`` (fn t => REWRITE_TAC [REWRITE_RULE [riscv_bmr_rel_EVAL] t] >> ASSUME_TAC t) >>
-`(∃mem_n.
+  `(?mem_n.
         bir_env_read (BVar "MEM8" (BType_Mem Bit64 Bit8)) bs.bst_environ =
-        SOME (BVal_Mem Bit64 Bit8 mem_n) ∧
-        ms.MEM8 = (λa. n2w (bir_load_mmap mem_n (w2n a))) ∧
-        bir_env_var_is_declared bs.bst_environ
-                                (BVar "tmp_MEM8" (BType_Mem Bit64 Bit8)))` by (
-                                METIS_TAC [riscv_bmr_rel_EVAL]
-                                ) >>
+        SOME (BVal_Mem Bit64 Bit8 mem_n) /\
+        ms.MEM8 = (\a. n2w (bir_load_mmap mem_n (w2n a))) /\
+        bir_env_var_is_declared bs.bst_environ (BVar "tmp_MEM8" (BType_Mem Bit64 Bit8)))`
+    by METIS_TAC [riscv_bmr_rel_EVAL] >>
   ASM_SIMP_TAC (std_ss) [] >>
-
   FULL_SIMP_TAC (std_ss++holBACore_ss++wordsLib.WORD_ss) [bir_immTheory.bool2b_def, bir_immTheory.bool2w_def] >>
-
   `bir_eval_bin_pred BIExp_Equal
                       (bir_eval_load (SOME (BVal_Mem Bit64 Bit8 mem_n))
                          (SOME (BVal_Imm (Imm64 pre_x10))) BEnd_LittleEndian
                          Bit64) (SOME (BVal_Imm (Imm64 pre_x10_mem_deref))) = SOME (BVal_Imm (Imm1 1w))` by (
-fs [type_of_bir_val_def,bir_eval_load_BASIC_REWR,type_of_bir_imm_def] >>
-  Cases_on `bir_load_from_mem Bit8 Bit64 Bit64 mem_n BEnd_LittleEndian (b2n (Imm64 pre_x10))` >- (
-    fs [bir_exp_memTheory.bir_load_from_mem_REWRS]
-  ) >>
+    fs [type_of_bir_val_def,bir_eval_load_BASIC_REWR,type_of_bir_imm_def] >>
+    Cases_on `bir_load_from_mem Bit8 Bit64 Bit64 mem_n BEnd_LittleEndian (b2n (Imm64 pre_x10))` >-
+     (fs [bir_exp_memTheory.bir_load_from_mem_REWRS]) >>
     FULL_SIMP_TAC (std_ss++holBACore_ss) [bir_eval_bin_pred_def] >>
-
-(**)
+    (**)
     fs [bir_exp_memTheory.bir_load_from_mem_REWRS] >>
-   POP_ASSUM (fn t => REWRITE_TAC [GSYM t]) >>
-  FULL_SIMP_TAC (std_ss++holBACore_ss) [] >>
-  (**)
-  REPEAT (PAT_X_ASSUM ``B1 @@ B2 @@ B3 @@ B4 @@ B5 @@ B6 @@ B7 @@ B8 = A`` (ASSUME_TAC o GSYM)) >>
-  ASM_REWRITE_TAC [] >>
-
-SIMP_TAC std_ss [bir_exp_memTheory.bir_mem_addr_w2n_SIZES, bir_exp_memTheory.bir_mem_addr_w2n_add_SIZES]    
-    
-  ) >>
+    POP_ASSUM (fn t => REWRITE_TAC [GSYM t]) >>
+    FULL_SIMP_TAC (std_ss++holBACore_ss) [] >>
+    (**)
+    REPEAT (PAT_X_ASSUM ``B1 @@ B2 @@ B3 @@ B4 @@ B5 @@ B6 @@ B7 @@ B8 = A`` (ASSUME_TAC o GSYM)) >>
+    ASM_REWRITE_TAC [] >>
+    SIMP_TAC std_ss [bir_exp_memTheory.bir_mem_addr_w2n_SIZES, bir_exp_memTheory.bir_mem_addr_w2n_add_SIZES]) >>
   `bir_eval_bin_pred BIExp_Equal
-                         (bir_eval_load (SOME (BVal_Mem Bit64 Bit8 mem_n))
-                            (SOME (BVal_Imm (Imm64 pre_x11)))
-                            BEnd_LittleEndian Bit64)
-                         (SOME (BVal_Imm (Imm64 pre_x11_mem_deref))) = SOME (BVal_Imm (Imm1 1w))` by (
-
-fs [type_of_bir_val_def,bir_eval_load_BASIC_REWR,type_of_bir_imm_def] >>
-  Cases_on `bir_load_from_mem Bit8 Bit64 Bit64 mem_n BEnd_LittleEndian (b2n (Imm64 pre_x11))` >- (
-    fs [bir_exp_memTheory.bir_load_from_mem_REWRS]
-  ) >>
+   (bir_eval_load (SOME (BVal_Mem Bit64 Bit8 mem_n))
+                  (SOME (BVal_Imm (Imm64 pre_x11)))
+                  BEnd_LittleEndian Bit64)
+   (SOME (BVal_Imm (Imm64 pre_x11_mem_deref))) = SOME (BVal_Imm (Imm1 1w))` by (
+    fs [type_of_bir_val_def,bir_eval_load_BASIC_REWR,type_of_bir_imm_def] >>
+    Cases_on `bir_load_from_mem Bit8 Bit64 Bit64 mem_n BEnd_LittleEndian (b2n (Imm64 pre_x11))` >-
+     (fs [bir_exp_memTheory.bir_load_from_mem_REWRS]) >>
     FULL_SIMP_TAC (std_ss++holBACore_ss) [bir_eval_bin_pred_def] >>
-
-(**)
+    (**)
     fs [bir_exp_memTheory.bir_load_from_mem_REWRS] >>
-   POP_ASSUM (fn t => REWRITE_TAC [GSYM t]) >>
-  FULL_SIMP_TAC (std_ss++holBACore_ss) [] >>
-  (**)
-  REPEAT (PAT_X_ASSUM ``B1 @@ B2 @@ B3 @@ B4 @@ B5 @@ B6 @@ B7 @@ B8 = A`` (ASSUME_TAC o GSYM)) >>
-  ASM_REWRITE_TAC [] >>
-
-SIMP_TAC std_ss [bir_exp_memTheory.bir_mem_addr_w2n_SIZES, bir_exp_memTheory.bir_mem_addr_w2n_add_SIZES]    
-
-
-    ) >>
-
+    POP_ASSUM (fn t => REWRITE_TAC [GSYM t]) >>
+    FULL_SIMP_TAC (std_ss++holBACore_ss) [] >>
+    (**)
+    REPEAT (PAT_X_ASSUM ``B1 @@ B2 @@ B3 @@ B4 @@ B5 @@ B6 @@ B7 @@ B8 = A`` (ASSUME_TAC o GSYM)) >>
+    ASM_REWRITE_TAC [] >>
+    SIMP_TAC std_ss [bir_exp_memTheory.bir_mem_addr_w2n_SIZES, bir_exp_memTheory.bir_mem_addr_w2n_add_SIZES]) >>
   FULL_SIMP_TAC (std_ss++holBACore_ss++wordsLib.WORD_ss) [bir_val_true_def]
-(*
-  IMP_RES_TAC bir_env_oldTheory.bir_env_var_is_initialised_weaken >>
-  FULL_SIMP_TAC (std_ss) [bir_env_oldTheory.bir_env_var_is_declared_def, GSYM bir_envTheory.bir_env_check_type_def] >>
-  ASM_SIMP_TAC (std_ss) [bir_envTheory.bir_env_read_def] >>
-*)
-(*
-
-
-  [,
-  bir_envTheory.bir_env_lookup_type_def, bir_envTheory.bir_env_lookup_def,bir_eval_bin_pred_def] >>
-
-FULL_SIMP_TAC (std_ss++holBACore_ss) [bir_envTheory.bir_env_read_def, bir_envTheory.bir_env_check_type_def,
-  bir_envTheory.bir_env_lookup_type_def, bir_envTheory.bir_env_lookup_def,bir_eval_bin_pred_def] >>
- cheat
-*)
 QED
 
-Theorem swap_riscv_post_imp_bir_post_thm:
+Theorem swap_riscv_post_imp_bspec_post_thm:
  !ls. bir_post_bir_to_riscv
    (riscv_swap_post pre_x10 pre_x11 pre_x10_mem_deref pre_x11_mem_deref)
-   (\l. (bir_swap_post pre_x10 pre_x11 pre_x10_mem_deref pre_x11_mem_deref))
+   (\l. (bspec_swap_post pre_x10 pre_x11 pre_x10_mem_deref pre_x11_mem_deref))
    ls
 Proof
- rw [bir_post_bir_to_riscv_def,riscv_swap_post_def,bir_swap_post_def,riscv_mem_load_dword_def] >>
+ rw [bir_post_bir_to_riscv_def,riscv_swap_post_def,bspec_swap_post_def,riscv_mem_load_dword_def] >>
  Cases_on `bs` >>
  Cases_on `b0` >>
  FULL_SIMP_TAC (std_ss++holBACore_ss) [bir_envTheory.bir_env_read_def, bir_envTheory.bir_env_check_type_def,
